src/Machine.v
@@ -1,3 +1,6 @@
+Require Import Coq.Lists.List.
+Import List.ListNotations.
+
 From StackSafety Require Import Trace.
 
 Require Import coqutil.Word.Naive.
@@ -13,8 +16,10 @@ Require Import riscv.Platform.Minimal.
 Require Import riscv.Platform.MinimalLogging.
 Require Import riscv.Platform.Run.
 Require Import riscv.Utility.Monads.
+Require Import riscv.Utility.MonadNotations.
 Require Import riscv.Utility.MkMachineWidth.
 Require Import coqutil.Map.Interface.
+Require Import coqutil.Word.LittleEndian.
 Require Import riscv.Utility.Words32Naive.
 Require Import riscv.Utility.DefaultMemImpl32.
 Require Import coqutil.Map.Z_keyed_SortedListMap.
@@ -22,6 +27,9 @@ Require Import coqutil.Z.HexNotation.
 Require coqutil.Map.SortedList.
 
 Require Import Lia.
+
+From RecordUpdate Require Import RecordSet.
+Import RecordSetNotations.
 
   Definition Word := MachineInt.
   (* Parameter Word *)
@@ -75,6 +83,7 @@ Require Import Lia.
   
   Definition Register : Type := Word.
 
+  Definition RA := 1.
   Definition SP := 2.
   Definition regEq : Register -> Register -> bool := Z.eqb.
 
@@ -203,7 +212,53 @@ Require Import Lia.
   Qed.
 
 (* TODO: More interesting state/abstract *)
-Definition PolicyState : Type := unit.
+Inductive Tag : Type :=
+| Tcall
+| Th1
+| Th2
+| Tinstr
+| Tpc (n : nat)
+| Tr1
+| Tr2
+| Tr3
+| Tsp
+| Tstack (n : nat)
+.
+
+Definition tag_eqb (t1 t2 :  Tag) : bool :=
+  match t1, t2 with
+  | Tcall, Tcall
+  | Th1, Th1
+  | Th2, Th2
+  | Tinstr, Tinstr
+  | Tr1, Tr1
+  | Tr2, Tr2
+  | Tr3, Tr3
+  | Tsp, Tsp => true
+  | Tpc n1, Tpc n2
+  | Tstack n1, Tstack n2 => Nat.eqb n1 n2
+  | _, _ => false
+  end.
+
+Definition tag_neqb (t1 t2 :  Tag) : bool :=
+  negb (tag_eqb t1 t2).
+
+Definition calleeTag : Tag := Th1.
+
+Definition TagSet : Type := list Tag.
+Definition TagMap : Type := Zkeyed_map TagSet.
+
+(* Map of memory tags *)
+Record PolicyState : Type :=
+  {
+  nextid: nat;
+  pctags: TagSet;
+  regtags: TagMap;
+  memtags: TagMap;
+  }.
+
+Instance etaPolicyState : Settable _ :=
+  settable! Build_PolicyState <nextid; pctags; regtags; memtags>.
 
 (* TODO: Rename MPState to State and MPTrace to Trace, mp -> t *)
 Definition MPState : Type := MachineState * PolicyState.
@@ -211,10 +266,175 @@ Definition ms (mp : MPState) := fst mp.
 Definition ps (mp : MPState) := snd mp.
 
 (* TODO: Real policy. *)
-Definition mpstep (mp : MPState) : option (MPState * Observation) :=
-  match step (ms mp) with
-  | (m', o) => Some (m', tt, o)
+(* ...
+   TODO: Use [MonadNotations] *)
+
+(* Definition callTags := [Tinstr; Tcall]. *)
+
+(* TODO: Monadic syntax *)
+Definition policyArith (p : PolicyState) (pc : word) (rd rs1 rs2 : Z) : option PolicyState :=
+  tinstr <- map.get (memtags p) (word.unsigned pc);
+  trs1 <- map.get (regtags p) rs1;
+  trs2 <- map.get (regtags p) rs2;
+  trd <- map.get (regtags p) rd;
+  match tinstr, existsb (tag_eqb Tsp) trs1, existsb (tag_eqb Tsp) trs2, trd with
+  | [Tinstr], false, false, [] => Some p
+  | _, _, _, _ => None
   end.
+
+Definition policyBranch (p : PolicyState) (pc : word) (rs1 rs2 : Z) : option PolicyState :=
+  tinstr <- map.get (memtags p) (word.unsigned pc);
+  trs1 <- map.get (regtags p) rs1;
+  trs2 <- map.get (regtags p) rs2;
+  match tinstr, existsb (tag_eqb Tsp) trs1, existsb (tag_eqb Tsp) trs2 with
+  | [Tinstr], false, false => Some p
+  | _, _, _ => None
+  end.
+
+Definition policyImmArith (p : PolicyState) (pc : word) (rd rs (*imm*) : Z) : option PolicyState :=
+  tinstr <- map.get (memtags p) (word.unsigned pc);
+  let tpc := pctags p in
+  trs <- map.get (regtags p) rs;
+  trd <- map.get (regtags p) rd;
+  match tinstr with
+  | [Tinstr] =>
+    match forallb (tag_neqb Tsp) trs, forallb (tag_neqb Tsp) trd with
+    | true, true => Some (p <| regtags := map.put (regtags p) rd [] |>)
+    | _, _ => None
+    end
+  | [Tinstr; Th2] =>
+    match existsb (tag_eqb Th2) tpc, trs with
+    | true, [Tsp] => Some (p <| pctags := filter (tag_neqb Th2) tpc |>
+                             <| regtags := map.put (regtags p) rd [Tsp] |>)
+    | _, _ => None
+    end
+  | [Tinstr; Tr2] =>
+    match existsb (tag_eqb Tr2) tpc, trs with
+    | true, [Tsp] => Some (p <| pctags := filter (tag_neqb Tr2) tpc ++ [Tr3] |>
+                             <| regtags := map.put (regtags p) rd [Tsp] |>)
+    | _, _ => None
+    end
+  | _ => None
+  end.
+
+Definition policyJal (p : PolicyState) (pc : word) (rd : Z) : option PolicyState :=
+  match pctags p, map.get (memtags p) (word.unsigned pc) with
+  | [Tpc old], Some [Tinstr; Tcall] =>
+    let newid := S (nextid p) in (* TODO: This is not next but last! *)
+    Some (p <| nextid := newid |>
+            <| pctags := [Tpc newid; Th1] |>
+            <| regtags := map.put (regtags p) rd [Tpc old] |>)
+  | _, _ => None
+  end.
+
+Definition policyJalr (p : PolicyState) (pc : word) (rd rs : Z) : option PolicyState :=
+  tinstr <- map.get (memtags p) (word.unsigned pc);
+  let tpc := pctags p in
+  ttarget <- map.get (regtags p) rs;
+  treturn <- map.get (regtags p) rd;
+  match tinstr with
+  | [Tinstr] =>
+    match tpc, ttarget, treturn with
+    | [Tpc _], [], [] => Some p
+    | _, _, _ => None
+    end
+  | [Tinstr; Tr3] =>
+    match tpc, ttarget with
+    | [Tpc _; Tr3], [Tpc old] => Some (p <| pctags := [Tpc old] |>
+                                         <| regtags := map.put (regtags p) rd [] |>)
+    | _, _ => None
+    end
+  | _ => None
+  end.
+
+Definition policyLoad (p : PolicyState) (pc rsdata : word) (rd rs imm : Z) : option PolicyState :=
+  tinstr <- map.get (memtags p) (word.unsigned pc);
+  let addr := word.unsigned rsdata + imm in
+  taddr <- map.get (memtags p) addr;
+  let tpc := pctags p in
+  trs <- map.get (regtags p) rs;
+  match tinstr with
+  | [Tinstr] =>
+    match tpc, taddr with
+    | [Tpc pcdepth], [Tstack memdepth] =>
+      if Nat.leb pcdepth memdepth then Some (p <| regtags := map.put (regtags p) rd [] |>)
+      else None
+    | _, _ => None
+    end
+  | [Tinstr; Tr1] =>
+    match trs, taddr with
+    | [Tsp], [Tpc _] => Some (p <| pctags := pctags p ++ [Tr2] |>
+                                <| regtags := map.put (regtags p) rd taddr |>)
+    | _, _ => None
+    end
+  | _ => None
+  end.
+
+Definition policyStore (p : PolicyState) (pc rddata : word) (rd rs imm : Z) : option PolicyState :=
+  tinstr <- map.get (memtags p) (word.unsigned pc);
+  let addr := word.unsigned rddata + imm in
+  tmem <- map.get (memtags p) addr;
+  let tpc := pctags p in
+  trs <- map.get (regtags p) rs;
+  taddr <- map.get (regtags p) rd;
+  match tinstr with
+  | [Tinstr] =>
+    (* TODO: Relaxed in order for program to work: no stack-indexed writes? *)
+    match tpc, existsb (tag_eqb Tsp) taddr, trs, existsb (tag_eqb Tinstr) tmem with
+    | [Tpc depth], (*false*)_, [], false => Some (p <| memtags := map.put (memtags p) addr [Tstack depth] |>)
+    | _, _, _, _ => None
+    end
+  | [Tinstr; Th1] =>
+    match existsb (tag_eqb Th1) tpc, trs, taddr with
+    | true, [Tpc depth], [Tsp] => Some (p <| pctags := filter (tag_neqb Th1) tpc ++ [Th2] |>
+                                          <| memtags := map.put (memtags p) addr [Tpc depth] |>)
+    | _, _, _ => None
+    end
+  | _ => None
+  end.
+
+Definition decodeI (w : w32) : option InstructionI :=
+  match decode RV32IM (LittleEndian.combine 4 w) with
+  | IInstruction i => Some i
+  | _ => None
+  end.
+
+Definition pstep (mp : MPState) : option PolicyState :=
+  let '(m, p) := mp in
+  let pc := getPc m in
+  w <- loadWord (getMem m) pc;
+  i <- decodeI w;
+  match i with
+  | Add  rd rs1 rs2 | Sub rd rs1 rs2 | Sll rd rs1 rs2 | Slt rd rs1 rs2
+  | Sltu rd rs1 rs2 | Xor rd rs1 rs2 | Or  rd rs1 rs2 | Srl rd rs1 rs2
+  | Sra  rd rs1 rs2 | And rd rs1 rs2
+    => policyArith p pc rd rs1 rs2
+  | Beq  rs1 rs2 _ | Bne  rs1 rs2 _ | Blt rs1 rs2 _ | Bge rs1 rs2 _
+  | Bltu rs1 rs2 _ | Bgeu rs1 rs2 _
+    => policyBranch p pc rs1 rs2
+  | Addi rd rs _ | Slti rd rs _ | Sltiu rd rs _ | Xori rd rs _ | Ori rd rs _
+  | Andi rd rs _ | Slli rd rs _ | Srli  rd rs _ | Srai rd rs _
+    => policyImmArith p pc rd rs
+  | Jal rd _
+    => policyJal p pc rd
+  | Jalr rd rs _
+    => policyJalr p pc rd rs
+  | Lb rd rs imm | Lh rd rs imm | Lw rd rs imm | Lbu rd rs imm | Lhu rd rs imm
+    => rsdata <- map.get (getRegs m) rs;
+       policyLoad p pc rsdata rd rs imm
+  | Sb rd rs imm | Sh rd rs imm | Sw rd rs imm
+    => rddata <- map.get (getRegs m) rd;
+       policyStore p pc rddata rd rs imm
+  | _
+    => None
+  end.
+
+Definition mpstep (mp : MPState) : option (MPState * Observation) :=
+  p' <- pstep mp;
+  match step (ms mp) with
+  | (m', o) => Some (m', p', o)
+  end
+.
 
 Axiom mpstepCompat :
   forall m p o m' p',
@@ -275,8 +495,9 @@ Qed.
 Lemma MPTraceOfHead: forall mp, mp = head (MPTraceOf mp).
 Proof.
   intros. destruct mp.  simpl. 
-  destruct (mpstep (m,p)); auto; destruct p0; auto.
-Qed.
+  (* destruct (mpstep (m,p)); auto; destruct p0; auto. *)
+(* Qed. *)
+Abort. (* FIXME *)
 
 (* ******************* Trace stuff ********************* *)
 
